Compiler proofs down to MC

driver/Compiler.v
@@ -83,6 +83,8 @@ Require FlatAsmGlobenv.
 Require FlatAsmProgram.
 Require FlatAsmgen.
 Require FlatAsmSep.
+Require MCgenproof.
+Require MCSep.
 (** Command-line flags. *)
 Require Import Compopts.
 
@@ -326,7 +328,14 @@ Definition flat_asm_passes :=
 
 Definition match_prog_flat := 
   pass_match (compose_passes (passes_app CompCert's_passes flat_asm_passes)).
-  
+
+Definition mc_passes :=
+  passes_app flat_asm_passes
+             (mkpass MCgenproof.match_prog ::: pass_nil _).
+
+Definition match_prog_mc := 
+  pass_match (compose_passes (passes_app CompCert's_passes mc_passes)).
+
 
 (** The [transf_c_program] function, when successful, produces
   assembly code that is in the [match_prog] relation with the source C program. *)
@@ -419,8 +428,10 @@ Theorem transf_c_program_flat_match:
     transf_c_program_flatasm p = OK tp ->
     match_prog_flat p tp.
 Proof.
-  intros p tp T. unfold transf_c_program_flatasm in T.
-  destruct (transf_c_program_real p) as [p1|e] eqn:TP; simpl in T; try discriminate. unfold time in T.
+  intros p tp T.
+  unfold transf_c_program_flatasm in T.
+  destruct (transf_c_program_real p) as [p1|e] eqn:TP; simpl in T; try discriminate.
+  unfold time in T.
   unfold match_prog_flat.
   rewrite compose_passes_app.
   apply transf_c_program_real_match in TP.
@@ -430,10 +441,32 @@ Proof.
   exists pi1; split; auto.
   unfold flat_asm_passes. simpl. 
   unfold real_asm_passes in CPR. simpl in CPR.
-  destruct CPR as (p2 & PM & p3 & PIM & EQ). subst.
+  destruct CPR as (p3 & PM & p4 & PIM & EQ). subst.
   eexists; split; eauto.
 Qed.
 
+Theorem transf_c_program_mc_match:
+  forall p tp,
+    transf_c_program_mc p = OK tp ->
+    match_prog_mc p tp.
+Proof.
+  intros p tp T.
+  unfold transf_c_program_mc in T.
+  destruct (transf_c_program_flatasm p) as [p1|e] eqn:TP; simpl in T; try discriminate.
+  unfold time in T.
+  unfold match_prog_mc.
+  rewrite compose_passes_app.
+  apply transf_c_program_flat_match in TP.
+  unfold match_prog_flat in TP.
+  rewrite compose_passes_app in TP.
+  destruct TP as (pi1 & CP & CPR).
+  exists pi1; split; auto.
+  unfold mc_passes. simpl. 
+  unfold flat_asm_passes, real_asm_passes in CPR. simpl in CPR.
+  destruct CPR as (p3 & PM & p4 & PIM & p5 & FAG & EQ). subst.
+  eexists; split; eauto.
+  eexists; split; eauto.
+Qed.
 
 (** * Semantic preservation *)
 
@@ -498,6 +531,15 @@ Definition flat_fn_stack_requirements (tp: FlatAsm.program) (id: ident) : Z :=
     end
   end.
 
+Definition mc_fn_stack_requirements (tp: MC.program) (id: ident) : Z :=
+  match List.find (fun '(id',_,_) => ident_eq id id') (FlatAsmProgram.prog_defs tp) with
+  | None => 0
+  | Some (_, def, _) =>
+    match def with
+    | Some (Gfun (Internal f)) => FlatAsmProgram.fn_stacksize f
+    | _ => 0
+    end
+  end.
 
 Definition printable_oracle (tp: Asm.program) : list (ident * Z) :=
   fold_left (fun acc gd =>
@@ -857,6 +899,98 @@ Proof.
   eapply FlatAsm.semantics_determinate.
 Qed.
 
+Lemma mc_fn_stack_requirements_match: forall p tp
+    (FM: MCgenproof.match_prog p tp),
+    flat_fn_stack_requirements p = mc_fn_stack_requirements tp.
+Proof.
+  intros.
+  unfold flat_fn_stack_requirements, mc_fn_stack_requirements.
+  apply Axioms.extensionality. intro i.
+  unfold MCgenproof.match_prog, MCgen.transf_program in FM.
+  repeat destr_in FM. monadInv H0. revert EQ. simpl.
+  generalize (FlatAsmProgram.prog_defs p) x. clear.
+  induction l; simpl; intros; eauto. inv EQ. simpl. auto.
+  monadInv EQ. specialize (IHl _ EQ).
+  destruct a. destruct p0. simpl. simpl in EQ0.
+  destruct x0. destruct p0.
+  assert (i0 = i1). repeat destr_in EQ0. monadInv H0. auto. subst.
+  destruct (ident_eq i i1). simpl.
+  repeat destr_in EQ0; auto. monadInv H0; auto.
+  unfold MCgen.transl_fun in EQ0. monadInv EQ0; simpl. auto.
+  simpl. auto.
+Qed.
+
+Lemma flatasmgen_update_maps_lmap_code:
+  forall defs g l d c g' l' d' c',
+    FlatAsmgen.update_maps g l d c defs = (g', l', d', c') ->
+    (forall i lb sb o, l i lb = Some (sb, o) -> sb = FlatAsmProgram.code_segid) ->
+    forall i lb sb o,
+      l' i lb = Some (sb, o) -> sb = FlatAsmProgram.code_segid.
+Proof.
+  intros defs g l d c g' l' d' c' H H0.
+  change ((fun g l d c =>
+           forall (i lb : ident) (sb : Segment.segid_type) (o : Integers.Ptrofs.int),
+  l i lb = Some (sb, o) -> sb = FlatAsmProgram.code_segid
+) g' l' d' c').
+  eapply FlatAsmgenproof.umind. eauto. auto.
+  clear. intros.
+  unfold FlatAsmgen.update_maps_def in H.
+  repeat destr_in H; eauto.
+  clear H1. revert l c i l' z Heqp H0 H2.
+  generalize (Asm.fn_code f0). clear.
+  induction c; simpl; intros; eauto. inv Heqp. eauto.
+  rewrite FlatAsmgenproof.update_instrs_cons in Heqp. destr_in Heqp.
+  specialize (IHc _ _ _ _ _ Heqp).
+  eapply IHc; eauto.
+  clear - Heqp0 H0.
+  unfold FlatAsmgen.update_instr in Heqp0. inv Heqp0. intros. destr_in H.
+  unfold FlatAsmgen.update_label_map in H. repeat destr_in H; eauto.
+  eauto.
+Qed.
+
+Lemma flatasmgen_make_maps_code:
+  forall p g l d c,
+    FlatAsmgen.make_maps p = (g, l, d, c) ->
+    forall i lb sb o,
+      l i lb = Some (sb, o) -> sb = FlatAsmProgram.code_segid.
+Proof.
+  unfold FlatAsmgen.make_maps.
+  intros. eapply flatasmgen_update_maps_lmap_code; eauto. unfold FlatAsmgen.default_label_map.
+  congruence.
+Qed.
+
+Theorem c_semantic_preservation_mc:
+  forall p tp,
+    match_prog_mc p tp ->
+    backward_simulation (Csem.semantics (mc_fn_stack_requirements tp) p) (MC.semantics tp (Asm.Pregmap.init Values.Vundef)).
+Proof.
+  intros.
+  unfold match_prog_mc in H.
+  unfold mc_passes in H.
+  rewrite compose_passes_app in H. 
+  destruct H as (pi & MP & P).
+  rewrite compose_passes_app in P.
+  destruct P as (pi' & RP & FP). simpl in FP.
+  destruct FP as (p2 & FP & EQ). subst p2.
+  assert (match_prog_flat p pi'). red. 
+  apply compose_passes_app. eexists; split; eauto.
+  eapply compose_backward_simulation.
+  apply MC.single_events.
+  replace (mc_fn_stack_requirements tp) with (flat_fn_stack_requirements pi').
+  apply c_semantic_preservation_flat; auto.
+  apply mc_fn_stack_requirements_match; auto.
+  eapply forward_to_backward_simulation.
+  eapply MCgenproof.transf_program_correct; eauto.
+  unfold flat_asm_passes in RP. simpl in RP.
+  destruct RP as (p2 & PI & p3 & PIP & p4 & FAP & EQ). subst.
+  unfold FlatAsmgenproof.match_prog, FlatAsmgen.transf_program in FAP.
+  repeat destr_in FAP. unfold FlatAsmgen.transl_prog_with_map in H1. monadInv H1. simpl.
+  clear - Heqp0. eapply flatasmgen_make_maps_code; eauto.
+  eapply FlatAsm.flat_asm_receptive.
+  eapply MC.semantics_determinate.
+Qed.
+
+
 
 
 (** * Correctness of the CompCert compiler *)
@@ -903,6 +1037,15 @@ Theorem transf_c_program_correct_flat:
 Proof.
   intros. apply c_semantic_preservation_flat. apply transf_c_program_flat_match; auto.
 Qed.
+
+Theorem transf_c_program_correct_mc:
+  forall p tp,
+    transf_c_program_mc p = OK tp ->
+    backward_simulation (Csem.semantics (mc_fn_stack_requirements tp) p) (MC.semantics tp (Asm.Pregmap.init Values.Vundef)).
+Proof.
+  intros. apply c_semantic_preservation_mc. apply transf_c_program_mc_match; auto.
+Qed.
+
 
 (** Here is the separate compilation case.  Consider a nonempty list [c_units]
   of C source files (compilation units), [C1 ,,, Cn].  Assume that every
@@ -998,6 +1141,26 @@ Proof.
   exists asm_program; split; auto. apply c_semantic_preservation_flat; auto.
 Qed.
 
+Theorem separate_transf_c_program_correct_mc:
+  forall c_units asm_units c_program,
+  nlist_forall2 (fun cu tcu => transf_c_program_mc cu = OK tcu) c_units asm_units ->
+  link_list c_units = Some c_program ->
+  exists asm_program, 
+      link_list asm_units = Some asm_program
+      /\
+      let init_stk := mk_init_stk_flat asm_program in
+      backward_simulation (Csem.semantics (mc_fn_stack_requirements asm_program) c_program) (MC.semantics asm_program
+                                                                                                           (Asm.Pregmap.init Values.Vundef)
+                                                                                         ).
+Proof.
+  intros. 
+  assert (nlist_forall2 match_prog_mc c_units asm_units).
+  { eapply nlist_forall2_imply. eauto. simpl; intros. apply transf_c_program_mc_match; auto. }
+  assert (exists asm_program, link_list asm_units = Some asm_program /\ match_prog_mc c_program asm_program).
+  { eapply link_list_compose_passes; eauto. }
+  destruct H2 as (asm_program & P & Q).
+  exists asm_program; split; auto. apply c_semantic_preservation_mc; auto.
+Qed.
 
 End WITHEXTERNALCALLS.
 
